verified/pagedb.s.dfy
@@ -1,4 +1,4 @@
-include "kev_constants.s.dfy"
+include "kev_common.s.dfy"
 include "Maybe.dfy"
 
 type PageNr = int
